code/k256/Hacl.K256.Scalar.fsti
@@ -17,9 +17,6 @@ module F = Hacl.K256.Field
 
 #set-options "--z3rlimit 50 --fuel 0 --ifuel 0"
 
-(**
-  This is a naive implementation of field arithmetic for testing purposes
-*)
 
 inline_for_extraction noextract
 let qnlimb = 4ul
@@ -67,6 +64,13 @@ val create_qelem: unit -> StackInline qelem
     qas_nat h1 f == 0)
 
 
+val is_qelem_zero (f:qelem) : Stack uint64
+  (requires fun h -> live h f)
+  (ensures  fun h0 m h1 -> modifies0 h0 h1 /\
+    (v m = 0 \/ v m = ones_v U64) /\
+    v m == (if qas_nat h0 f = 0 then ones_v U64 else 0))
+
+
 val is_qelem_zero_vartime (f:qelem) : Stack bool
   (requires fun h -> live h f)
   (ensures  fun h0 m h1 -> modifies0 h0 h1 /\
@@ -82,8 +86,7 @@ val is_qelem_eq_vartime (f1 f2:qelem) : Stack bool
 
 val load_qelem: f:qelem -> b:lbuffer uint8 32ul -> Stack unit
   (requires fun h ->
-    live h f /\ live h b /\ disjoint f b /\
-    BSeq.nat_from_bytes_be (as_seq h b) < S.q)
+    live h f /\ live h b /\ disjoint f b)
   (ensures  fun h0 _ h1 -> modifies (loc f) h0 h1 /\
     qas_nat h1 f == BSeq.nat_from_bytes_be (as_seq h0 b))
 
