code/k256/Hacl.Spec.K256.Field52.fst
@@ -80,34 +80,6 @@ let is_felem_ge_prime5 ((t0,t1,t2,t3,t4): felem5) : uint64 =
 
 
 inline_for_extraction noextract
-let is_felem_lt_vartime5 ((a0,a1,a2,a3,a4): felem5) ((b0,b1,b2,b3,b4): felem5) : bool =
-  let open Lib.RawIntTypes in
-  if u64_to_UInt64 a4 <. u64_to_UInt64 b4 then true
-  else begin
-    if u64_to_UInt64 a4 >. u64_to_UInt64 b4 then false
-    else begin
-      if u64_to_UInt64 a3 <. u64_to_UInt64 b3 then true
-      else begin
-        if u64_to_UInt64 a3 >. u64_to_UInt64 b3 then false
-        else begin
-          if u64_to_UInt64 a2 <. u64_to_UInt64 b2 then true
-          else begin
-            if u64_to_UInt64 a2 >. u64_to_UInt64 b2 then false
-            else begin
-              if u64_to_UInt64 a1 <. u64_to_UInt64 b1 then true
-              else begin
-                if u64_to_UInt64 a1 >. u64_to_UInt64 b1 then false
-                else u64_to_UInt64 a0 <. u64_to_UInt64 b0
-              end
-            end
-          end
-        end
-      end
-    end
-  end
-
-
-inline_for_extraction noextract
 let is_felem_lt_prime_minus_order_vartime5 ((f0,f1,f2,f3,f4): felem5) : bool =
   let open Lib.RawIntTypes in
   if u64_to_UInt64 f4 >. 0uL then false
